pulse/lib/pulse/core/PulseCore.IndirectionTheorySep.fsti
@@ -163,9 +163,9 @@ val lift_pure_eq (p:prop) : Lemma (
 val lift_star_eq (p q:pm_slprop) : Lemma (
   lift (PM.star p q) == star (lift p) (lift q)
 )
-val lift_exists_eq (a:Type u#4) (f:a -> pm_slprop) : Lemma (
-  lift PM.(h_exists #a f) == (exists* (x:a). lift (f x))
-)
+// val lift_exists_eq (a:Type u#4) (f:a -> pm_slprop) : Lemma (
+//   lift PM.(h_exists #a f) == (exists* (x:a). lift (f x))
+// )
 
 (**** Memory invariants *)
 [@@erasable]
